@@ -38,7 +38,6 @@ import MachCSL.WpSmodeKpt
 import MachCSL.CallConv
 import MachCSL.WpSmodeFrame
 import MachCSL.WpSmodeFrame8
-import MachCSL.WpSmodeFrame6
 import MachCSL.WpStagesM
 import MachCSL.WpGpr
 import MachCSL.GprLit
